get_child_index...결국 'assume'를 사용했다...;;

src/study/Nemonuri.Study.CSharpSyntaxRewriter2.Modifier2/Nemonuri.StratifiedNodes.Common.fst
@@ -1,5 +1,7 @@
 module Nemonuri.StratifiedNodes.Common
 
+module L = FStar.List.Tot
+
 //--- type definitions ---
 let aggregator (t:Type) = (aggregated:t) -> (aggregating:t) -> t
 //---|
@@ -24,4 +26,23 @@ let rec take_while #t
   (predicate:t -> Tot bool)
   : Tot (list t) (decreases l) =
 *)
+
+// https://learn.microsoft.com/en-us/dotnet/api/system.collections.generic.list-1.findindex?view=net-9.0
+let rec find_index #t 
+  (l:list t) (predicate:t -> Tot bool)
+  : Pure nat 
+    (requires 
+      Some? (L.find predicate l)
+    )
+    (ensures fun r -> 
+      let v1 = L.length l in
+      (0 <= r) && (r < v1)
+    )
+    (decreases l)
+  =
+  let hd::tl = l in
+  match predicate hd with
+  | true -> 0
+  | false -> 1 + (find_index tl predicate)
+
 //---|
