src/study/Nemonuri.Study.CSharpSyntaxRewriter2.Modifier2/Nemonuri.StratifiedNodes.Indexes.fst
@@ -6,9 +6,23 @@ module C = Nemonuri.StratifiedNodes.Children
 module Common = Nemonuri.StratifiedNodes.Common
 
 //--- theory members ---
-let to_indexes #t (ancestors:C.ancestor_list t)
-  : Pure (list nat) (requires True) (ensures fun r -> true)
+private let rec to_indexes_core #t (hd:N.node t) (tl:C.ancestor_list t) 
+  : Pure (list nat) 
+    (requires (C.is_concatenatable_to_ancestor_list hd tl))
+    (ensures fun r -> true)
   =
-  ()
+  match tl with
+  | [] -> []
+  | hd2::tl2 -> 
+
+let to_indexes #t (ancestors:C.ancestor_list t)
+  : Pure (list nat) 
+    (requires (Cons? ancestors)) 
+    (ensures fun r -> true)
+  =
+  let hd::tl = ancestors in
+  match tl with
+  | [] -> []
+  | 
 
 //---|
